doc: Document relabelNat

LeanSAT/AIG/RelabelNat.lean
@@ -4,11 +4,22 @@ open Std
 
 variable {α : Type} [BEq α] [Hashable α]
 
+-- TODO: auxiliary theorem, possibly upstream
+theorem _root_.Array.get_of_mem {a : α} {as : Array α}
+    : a ∈ as → (∃ (i : Fin as.size), as[i] = a) := by
+  intro ha
+  rcases List.get_of_mem ha.val with ⟨i, hi⟩
+  exists i
+
 namespace AIG
-
 namespace RelabelNat
+namespace State
 
-inductive State.Inv1 : Nat → HashMap α Nat → Prop where
+/--
+This invariant ensures that we only insert an atom at most once and with a monotonically increasing
+index.
+-/
+inductive Inv1 : Nat → HashMap α Nat → Prop where
 | empty : Inv1 0 {}
 | insert (hinv : Inv1 n map) (hfind : map.find? x = none) : Inv1 (n + 1) (map.insert x n)
 
@@ -27,10 +38,13 @@ Proof sketch for this axiom once we have more `HashMap` theory:
     sorry
 ```
 -/
-axiom State.Inv1.property {n m : Nat} (x y : α) (map : HashMap α Nat) (hinv : State.Inv1 n map)
+axiom Inv1.property {n m : Nat} (x y : α) (map : HashMap α Nat) (hinv : Inv1 n map)
     (hfound1 : map.find? x = some m) (hfound2 : map.find? y = some m) : x = y
 
-inductive State.Inv2 (decls : Array (Decl α)) : Nat → HashMap α Nat → Prop where
+/--
+This invariant says that we have already visited and inserted all nodes up to a certain index.
+-/
+inductive Inv2 (decls : Array (Decl α)) : Nat → HashMap α Nat → Prop where
 | empty : Inv2 decls 0 {}
 | newAtom (hinv : Inv2 decls idx map) (hlt : idx < decls.size) (hatom : decls[idx] = .atom a)
   (hmap : map.find? a = none)
@@ -43,27 +57,59 @@ inductive State.Inv2 (decls : Array (Decl α)) : Nat → HashMap α Nat → Prop
 | gate (hinv : Inv2 decls idx map) (hlt : idx < decls.size) (hatom : decls[idx] = .gate l r li ri)
   : Inv2 decls (idx + 1) map
 
-theorem State.Inv2.upper_lt_size {decls : Array (Decl α)} (hinv : Inv2 decls upper map)
+-- TODO: Think about merging Inv1 and Inv2, they are *very* close.
+
+theorem Inv2.upper_lt_size {decls : Array (Decl α)} (hinv : Inv2 decls upper map)
     : upper ≤ decls.size := by
   cases hinv <;> omega
 
-axiom State.Inv2.property (decls : Array (Decl α)) (idx upper : Nat) (map : HashMap α Nat)
+/--
+The key property provided by `Inv2`, if we have `Inv2` at a certain index, then all atoms below
+that index have been inserted into the `HashMap`.
+-/
+axiom Inv2.property (decls : Array (Decl α)) (idx upper : Nat) (map : HashMap α Nat)
     (hinv : Inv2 decls upper map)
     : ∀ (hidx : idx < upper), ∀ (a : α),
         decls[idx]'(by have := upper_lt_size hinv; omega) = .atom a
           → ∃ n, map.find? a = some n
 
+end State
+
+/--
+The invariant carrying state structure for building the `HashMap` that translates from arbitrary
+atom identifiers to `Nat`.
+-/
 structure State (α : Type) [BEq α] [Hashable α] (decls : Array (Decl α)) (idx : Nat) where
+  /--
+  The next number to use for identifying an atom.
+  -/
   max : Nat
+  /--
+  The translation `HashMap`
+  -/
   map : HashMap α Nat
+  /--
+  Proof that we never reuse a number.
+  -/
   inv1 : State.Inv1 max map
+  /--
+  Proof that we inserted all atoms until `idx`.
+  -/
   inv2 : State.Inv2 decls idx map
 
-def State.empty {decls : Array (Decl α)} : State α decls 0 :=
-  { max := 0, map := {}, inv1 := State.Inv1.empty, inv2 := State.Inv2.empty }
+namespace State
 
-def State.addVar {decls : Array (Decl α)} (state : State α decls idx) (a : α)
-    (h : decls[idx]'sorry = .atom a)
+/--
+The basic initial state.
+-/
+def empty {decls : Array (Decl α)} : State α decls 0 :=
+  { max := 0, map := {}, inv1 := Inv1.empty, inv2 := Inv2.empty }
+
+/--
+Insert a `Decl.atom` into the `State` structure.
+-/
+def addAtom {decls : Array (Decl α)} {hidx} (state : State α decls idx) (a : α)
+    (h : decls[idx]'hidx = .atom a)
     : State α decls (idx + 1) :=
   match hmap:state.map.find? a with
   | some _ =>
@@ -89,8 +135,11 @@ def State.addVar {decls : Array (Decl α)} (state : State α decls idx) (a : α)
         . assumption
     }
 
-def State.addConst {decls : Array (Decl α)} (state : State α decls idx) (b : Bool)
-    (h : decls[idx]'sorry = .const b)
+/--
+Insert a `Decl.const` into the `State` structure.
+-/
+def addConst {decls : Array (Decl α)} {hidx} (state : State α decls idx) (b : Bool)
+    (h : decls[idx]'hidx = .const b)
     : State α decls (idx + 1) :=
   { state with
       inv2 := by
@@ -99,8 +148,11 @@ def State.addConst {decls : Array (Decl α)} (state : State α decls idx) (b : B
         . assumption
   }
 
-def State.addGate {decls : Array (Decl α)} (state : State α decls idx) (lhs rhs : Nat)
-    (linv rinv : Bool) (h : decls[idx]'sorry = .gate lhs rhs linv rinv)
+/--
+Insert a `Decl.gate` into the `State` structure.
+-/
+def addGate {decls : Array (Decl α)} {hidx} (state : State α decls idx) (lhs rhs : Nat)
+    (linv rinv : Bool) (h : decls[idx]'hidx = .gate lhs rhs linv rinv)
     : State α decls (idx + 1) :=
   { state with
       inv2 := by
@@ -109,14 +161,17 @@ def State.addGate {decls : Array (Decl α)} (state : State α decls idx) (lhs rh
         . assumption
   }
 
-def State.ofAIGAux (aig : AIG α) : State α aig.decls aig.decls.size :=
-  go aig.decls 0 State.empty
+/--
+Build up a `State` that has all atoms of an `AIG` inserted.
+-/
+def ofAIGAux (aig : AIG α) : State α aig.decls aig.decls.size :=
+  go aig.decls 0 .empty
 where
   go (decls : Array (Decl α)) (idx : Nat) (state : State α decls idx) : State α decls decls.size :=
     if hidx:idx < decls.size then
       let decl := decls[idx]
       match hdecl:decl with
-      | .atom a => go decls (idx + 1) (state.addVar a hdecl)
+      | .atom a => go decls (idx + 1) (state.addAtom a hdecl)
       | .const b => go decls (idx + 1) (state.addConst b hdecl)
       | .gate lhs rhs linv rinv => go decls (idx + 1) (state.addGate lhs rhs linv rinv hdecl)
     else
@@ -126,26 +181,40 @@ where
       this ▸ state
   termination_by decls.size - idx
 
-def State.ofAIG (aig : AIG α) : HashMap α Nat :=
-  State.ofAIGAux aig |>.map
+/--
+Obtain the atom mapping from α to `Nat` for a given `AIG`.
+-/
+def ofAIG (aig : AIG α) : HashMap α Nat :=
+  ofAIGAux aig |>.map
 
-theorem State.ofAIG.Inv1 (aig : AIG α) : ∃ n, State.Inv1 n (State.ofAIG aig) := by
-  exists (State.ofAIGAux aig).max
+/--
+The map returned by `ofAIG` fulfills the `Inv1` property.
+-/
+theorem ofAIG.Inv1 (aig : AIG α) : ∃ n, Inv1 n (ofAIG aig) := by
+  exists (ofAIGAux aig).max
   dsimp [ofAIG]
-  exact (State.ofAIGAux aig).inv1
+  exact (ofAIGAux aig).inv1
 
-theorem State.ofAIG.Inv2 (aig : AIG α) : State.Inv2 aig.decls aig.decls.size (State.ofAIG aig) := by
-  have := (State.ofAIGAux aig).inv2
-  simp [State.ofAIG, this]
+/--
+The map returned by `ofAIG` fulfills the `Inv2` property.
+-/
+theorem ofAIG.Inv2 (aig : AIG α) : Inv2 aig.decls aig.decls.size (ofAIG aig) := by
+  have := (ofAIGAux aig).inv2
+  simp [ofAIG, this]
 
--- TODO: auxiliary theorem, possibly upstream
-theorem _root_.Array.get_of_mem {a : α} {as : Array α}
-    : a ∈ as → (∃ (i : Fin as.size), as[i] = a) := by
-  intro ha
-  rcases List.get_of_mem ha.val with ⟨i, hi⟩
-  exists i
+/--
+Assuming that we find a `Nat` for an atom in the `ofAIG` map, that `Nat` is unique in the map.
+-/
+theorem ofAIG_find_unique {aig : AIG α} (a : α) (ha : (ofAIG aig).find? a = some n)
+    : ∀ a', (ofAIG aig).find? a' = some n → a = a' := by
+  intro a' ha'
+  rcases ofAIG.Inv1 aig with ⟨n, hn⟩
+  apply Inv1.property <;> assumption
 
-theorem State.ofAIG_find_some {aig : AIG α} : ∀ a ∈ aig, ∃ n, (State.ofAIG aig).find? a = some n := by
+/--
+We will find a `Nat` for every atom in the `AIG` that the `ofAIG` map was built from.
+-/
+theorem ofAIG_find_some {aig : AIG α} : ∀ a ∈ aig, ∃ n, (ofAIG aig).find? a = some n := by
   intro a ha
   simp only [mem_def] at ha
   rcases Array.get_of_mem ha with ⟨⟨i, isLt⟩, hi⟩
@@ -155,14 +224,13 @@ theorem State.ofAIG_find_some {aig : AIG α} : ∀ a ∈ aig, ∃ n, (State.ofAI
   . apply ofAIG.Inv2
   . omega
 
-theorem State.ofAIG_find_unique {aig : AIG α} (a : α) (ha : (State.ofAIG aig).find? a = some n)
-    : ∀ a', (State.ofAIG aig).find? a' = some n → a = a' := by
-  intro a' ha'
-  rcases State.ofAIG.Inv1 aig with ⟨n, hn⟩
-  apply State.Inv1.property <;> assumption
-
+end State
 end RelabelNat
 
+/--
+Map an `AIG` with arbitrary atom identifiers to one that uses `Nat` as atom identifiers. This is
+useful for preparing an `AIG` for CNF translation if it doesn't already use `Nat` identifiers.
+-/
 def relabelNat (aig : AIG α) : AIG Nat :=
   let map := RelabelNat.State.ofAIG aig
   aig.relabel fun x =>
@@ -175,6 +243,9 @@ def relabelNat (aig : AIG α) : AIG Nat :=
 theorem relabelNat_size_eq_size {aig : AIG α} : aig.relabelNat.decls.size = aig.decls.size := by
   simp [relabelNat]
 
+/--
+`relabelNat` preserves unsatisfiablility.
+-/
 theorem relabelNat_unsat_iff [Nonempty α] {aig : AIG α} {hidx1} {hidx2}
     : (aig.relabelNat).unsatAt idx hidx1 ↔ aig.unsatAt idx hidx2 := by
   dsimp [relabelNat]
@@ -199,12 +270,20 @@ theorem relabelNat_unsat_iff [Nonempty α] {aig : AIG α} {hidx1} {hidx2}
 
 namespace Entrypoint
 
+/--
+Map an `Entrypoint` with arbitrary atom identifiers to one that uses `Nat` as atom identifiers.
+This is useful for preparing an `AIG` for CNF translation if it doesn't already use `Nat`
+identifiers.
+-/
 def relabelNat (entry : Entrypoint α) : Entrypoint Nat :=
   { entry with
       aig := entry.aig.relabelNat
       inv := by simp[entry.inv]
   }
 
+/--
+`relabelNat` preserves unsatisfiablility.
+-/
 theorem relabelNat_unsat_iff {entry : Entrypoint α} [Nonempty α]
     : (entry.relabelNat).unsat ↔ entry.unsat:= by
   simp [relabelNat, unsat]
